\subsection{Problem}

\renewcommand{\theequation}{\theenumi}
\begin{enumerate}[label=\thesection.\arabic*.,ref=\thesection.\theenumi]
\numberwithin{equation}{enumi}

	\item Find a quadratic polynomial each with the given numbers as the sum and the product of its zeroes.
	\begin{enumerate}
	
		\item -1,$\frac{1}{4}$
		\\
		\solution For a general polynomial equation of degree 2,
	\begin{multline}
	p\brak{x,y} \implies Ax^2 +Bxy + Cy^2 +Dx + Ey + F = 0\\
	\text{The vector form is}\\
	\vec{x}^T\myvec{A&\frac{B}{2}\\\frac{B}{2}&C}\vec{x}  + \myvec{D&E}\vec{x} + F = 0 \label{eq:qtwenty}
	\end{multline}
Here, sum of zeroes = D = -1\\
Product of zeroes = F =$\frac{1}{4}$\\
Substituing the values in \ref{eq:qtwenty},\\
\begin{multline}
\vec{x}^T\myvec{1&0\\0&0}\vec{x}  + 
\myvec{1&-1}\vec{x} +\frac{1}{4} = 0\\
\end{multline}
\begin{align}
\implies y = x^2 + x + \frac{1}{4}
\end{align}
	
		
		\item 1,1
		\\
		\solution
Here, sum of zeroes = D = 1\\
Product of zeroes = F =1\\
Substituing the values in \ref{eq:qtwenty},\\
\begin{multline}
\vec{x}^T\myvec{1&0\\0&0}\vec{x}  + \myvec{-1&-1}\vec{x} +1 = 0
\end{multline}
\begin{align}
\implies y = x^2 - x + 1 
\end{align}
		
		\item 0,$\sqrt{5}$\\
		\solution
Here, sum of zeroes = D = 0\\
Product of zeroes = F =$\sqrt{5}$\\
Substituing the values in \ref{eq:qtwenty},\\
\begin{multline}
\vec{x}^T\myvec{1&0\\0&0}\vec{x}  + \myvec{0&-1}\vec{x} + \sqrt{5} = 0
\end{multline}
\begin{align}
\implies y = x^2 + \sqrt{5}  
\end{align}
		\item 4,1\\
		\solution 
Here, sum of zeroes = D = 4\\
Product of zeroes = F = 1\\
Substituing the values in \ref{eq:qtwenty},\\
\begin{multline}
\vec{x}^T\myvec{1&0\\0&0}\vec{x}  + \myvec{-4&-1}\vec{x} + 1 = 0
\end{multline}
\begin{align}
\implies y = x^2 - 4x + 1 
\end{align}


		\item $\frac{1}{4}$,$\frac{1}{4}$\\
\solution 
Here, sum of zeroes = D = $\frac{1}{4}$\\
Product of zeroes = F = $\frac{1}{4}$\\
Substituing the values in \ref{eq:qtwenty},\\

\begin{multline}
\vec{x}^T\myvec{1&0\\0&0}\vec{x}  + \myvec{-\frac{1}{4}&-1}\vec{x} + \frac{1}{4} = 0
\end{multline}
\begin{align}
\implies y = x^2 - \frac{1}{4}x + \frac{1}{4} 
\end{align}


		\item $\sqrt{2}$,$\frac{1}{3}$\\
\solution
Here, sum of zeroes = D = $\sqrt{2}$\\
Product of zeroes = F = $\frac{1}{3}$\\
Substituing the values in \ref{eq:qtwenty},\\
\begin{multline}
\vec{x}^T\myvec{1&0\\0&0}\vec{x}  + \myvec{-\sqrt{2}&-1}\vec{x} + \frac{1}{3} = 0
\end{multline}
\begin{align}
\implies y = x^2 - \sqrt{2}x + \frac{1}{3}
\end{align}
	\end{enumerate}
\end{enumerate}
