\renewcommand{\vec}[1]{\mathbf{#1}}
 \renewcommand{\theequation}{\theenumi}
\begin{enumerate}[label=\thesection.\arabic*.,ref=\thesection.\theenumi]
\numberwithin{equation}{enumi}

 \item
 $\triangle EAD \sim \triangle BAO$ by AAA Similarity:

Since $\vec{DE} \parallel \vec{OB}$,
\begin{enumerate}
	\item $\angle{DEA} = \angle{OBA} \quad \brak{\text{Alternate Interior Angles}}$
	\item $\angle{ADE} = \angle{AOB} \quad \brak{\text{Alternate Interior Angles}}$
	  
	\item $\angle{EAD} = \angle{BAO} \quad \brak{\text{Common angle}} $
	
\end{enumerate}

Therefore 
\begin{align}
\vec{\frac{AE}{AB}} = \vec{\frac{AD}{AO}}
\end{align}

\item
Similarly 
$\triangle FDA \sim \triangle COA$ by AAA Similarity:

Since $\vec{DF} \parallel \vec{OC}$,
\begin{enumerate}
	\item $\angle{DFA} = \angle{OCA} \quad \brak{\text{Alternate Interior Angles}}$
	\item $\angle{ADF} = \angle{AOC} \quad \brak{\text{Alternate Interior Angles}}$
	  
	\item $\angle{FAD} = \angle{CAO} \quad \brak{\text{Common angle}} $
	
\end{enumerate}


Therefore 
\begin{align}
\vec{\frac{AF}{AC}} = \vec{\frac{AD}{AO}}
\end{align}


\item
Hence from the above we conclude,
\begin{align}
\vec{\frac{AF}{AC}} = \vec{\frac{AE}{AB}} = \vec{\frac{AD}{AO}}
\end{align}
\end{enumerate}
As the ratio of the sides is the same, $\triangle$ ABC $\sim \triangle$ AEF, which means $\angle{AFE} = \angle{ACB}$ and $\angle{AEF} = \angle{ABC}$ as similar triangles have same angles.
i.e. 

\begin{align}
\vec{EF} \parallel \vec{QR}
\end{align}
\begin{centering}
Hence Proved.
\end{centering}
